wip: projection machine

TM/Code/MatchTM.v
@@ -8,6 +8,8 @@ Require Import TM.Compound.TMTac.
 Require Import TM.Compound.CopySymbols TM.Compound.MoveToSymbol.
 
 
+Check ltac:(idtac "Warning: This file could take LONG!"; apply 42).
+
 
 (* Basic pattern matching *)
 Section MatchSum.
@@ -121,6 +123,248 @@ Section MatchSum.
   End SumConstr.
 
 End MatchSum.
+
+
+Section Copy.
+
+  Section Test.
+
+    Let inputX := encode (4, 3).
+    Compute inputX.
+
+    Let t : tape (Bool_Fin + Bool_Fin)^+ :=
+      midtape [inr START] (inl (inl true))
+              (map inl [inl true; inl true; inl true; inl false; 
+                          inr true; inr true; inr true; inr false] ++ [inr STOP; inl (inl true)]).
+
+    Compute tape_local t.
+    Let stop_X :=
+      fun (x : (Bool_Fin+Bool_Fin)^+) =>
+        match x with
+        | (inl (inl _)) => false
+        | _ => true (* Stop at symbol from Y or halt/stop symbol *)
+        end.
+
+    (* CopySymbols_Fun is not computable!  Use the equational rewriting to "execute"
+     * (CopSymbols_Fun can be made computable by changing the termination proof to Qed.)
+     *)
+    Goal True.
+      Ltac re x := assert (x = x) by reflexivity.
+      re (tape_local (fst (CopySymbols_Fun stop_X id (t, rightof (inr START) [])))).
+      re (snd (CopySymbols_Fun stop_X id (t, rightof (inr START) []))).
+      re ((left (snd (CopySymbols_Fun stop_X id (t, rightof (inr START) []))))).
+      subst t; repeat ( rewrite CopySymbols_Fun_equation in * || cbn in * ); cbv [id] in *.
+    Abort.
+    
+  End Test.
+  
+  (* Require Import FunInd. *)
+
+  Variable sig : finType.
+  Variable stop : sig -> bool.
+
+  Lemma CopySymbols_pair_first tltr str1 x str2 tl' tr':
+    (forall x, List.In x str1 -> stop x = false) ->
+    (stop x = true) ->
+    tape_local (fst tltr) = str1 ++ [x] ++ str2 ->
+    (tl', tr') = CopySymbols_Fun stop id tltr ->
+    tape_local tl' = x :: str2.
+  Proof.
+    intros H H0. destruct tltr as [tl tr]. intros H1 E0.
+    destruct tl as [ | r rs | l ls | ls m rs]; cbn in *.
+    1-3: rewrite CopySymbols_Fun_equation in E0; inv H1; exfalso; destruct str1; cbn in *; congruence.
+    revert rs tr ls H ls m H1 tl' tr' E0. revert str1; intros str1.
+    induction str1 as [ | s' str1' IHstr1]; (* cbn in *; *) intros.
+    - cbn in *. inv H1. rewrite CopySymbols_Fun_equation in E0. rewrite H0 in E0. inv E0. cbn. auto.
+    - rewrite CopySymbols_Fun_equation in E0. destruct (stop m) eqn:E1.
+      + inv E0. cbn in *. inv H1. enough (stop s' = false)  by congruence; eauto.
+      + cbn in H1. inv H1. cbn in *. destruct str1'; cbn in *; eapply IHstr1; eauto.
+  Qed.
+
+  Lemma CopySymbols_pair_second tltr str1 x str2 tl' tr':
+    (forall x, List.In x str1 -> stop x = false) ->
+    (stop x = true) ->
+    tape_local (fst tltr) = str1 ++ [x] ++ str2 ->
+    (tl', tr') = CopySymbols_Fun stop id tltr ->
+    left tr' = rev str1 ++ left (snd tltr).
+  Proof.
+    intros H H0. destruct tltr as [tl tr]. intros H1 E0.
+    destruct tl as [ | r rs | l ls | ls m rs]; cbn in *.
+    1-3: rewrite CopySymbols_Fun_equation in E0; inv H1; exfalso; destruct str1; cbn in *; congruence.
+    revert rs tr ls H ls m H1 tl' tr' E0. revert str1; intros str1.
+    induction str1 as [ | s' str1' IHstr1]; (* cbn in *; *) intros.
+    - cbn in *. inv H1. rewrite CopySymbols_Fun_equation in E0. rewrite H0 in E0. inv E0. cbn. auto.
+    - rewrite CopySymbols_Fun_equation in E0. destruct (stop m) eqn:E1.
+      + inv E0. cbn in *. inv H1. enough (stop s' = false)  by congruence; eauto.
+      + cbn in H1. inv H1. cbn in *.
+        simpl_list; cbn.
+        destruct str1'; cbn in *.
+        * clear H. erewrite IHstr1; eauto. destruct tr; cbn; eauto. destruct l0; cbn; auto.
+        * simpl_list; cbn.
+          erewrite IHstr1; eauto. destruct tr; simpl_list; cbn; eauto. destruct l0; cbn; auto.
+  Qed.
+
+
+  (*
+  Lemma MoveToSymbol_right t str1 str2 x :
+    (forall x, List.In x str1 -> stop x = false) ->
+    (exists s, current t = Some s) ->
+    (stop x = true) ->
+    right t = str1 ++ x :: str2 ->
+    right (MoveToSymbol_Fun stop t) = str2.
+  Proof.
+    intros H H0 H1. destruct t as [ | r rs | l ls | ls m rs]; cbn in *.
+    1,3: rewrite MoveToSymbol_Fun_equation; cbn; destruct str1; cbn in *; try congruence.
+    1: destruct H0; congruence.
+    1: clear H0.
+    revert rs m ls ls H1. induction str1 as [ | s' str1' IHstr1]; cbn in *; intros.
+    - rewrite MoveToSymbol_Fun_equation. cbn. destruct (stop m) eqn:E1.
+      + cbn.
+
+    
+    revert str1 str2 m ls H H1. induction rs as [ | r rs' IHl]; cbn in *; intros.
+    - destruct str1; cbn in *; congruence.
+    - rewrite MoveToSymbol_Fun_equation; cbn.
+      destruct (stop m) eqn:E1; cbn in *.
+      + destruct str1; cbn in *. inv H1.
+   *)
+    
+    
+  
+End Copy.
+
+
+
+Section Projection.
+
+  Variable X Y : Type.
+  Variable (sigX sigY : finType).
+  Hypothesis (codX : codeable sigX X) (codY : codeable sigY Y).
+
+
+  Definition stop_X :=
+    fun (x : (sigX+sigY)^+) =>
+      match x with
+      | (inl (inl _)) => false
+      | _ => true (* Stop at symbol from Y or halt/stop symbol *)
+      end.
+
+  Definition stop_Y :=
+    fun (x : (sigX+sigY)^+) =>
+      match x with
+        inl (inr _) => false
+      | _ => true (* Stop at symbol from X or halt/stop symbol *)
+      end.
+
+
+  Definition Proj_Rel : Rel (tapes (sigX+sigY)^+ 2) (unit * tapes (sigX+sigY)^+ 2) :=
+    ignoreParam (
+        fun (tin tout : tapes (sigX+sigY)^+ 2) =>
+          forall (xy : X * Y),
+            tape_encodes (Encode_Pair' codX codY) tin[@Fin.F1] xy ->
+            tape_encodes (Encode_Map codY (@retract_inr sigX sigY)) tout[@Fin.F1] (snd xy) /\
+            tape_encodes (Encode_Map codX (@retract_inl sigX sigY)) tout[@Fin.FS Fin.F1] (fst xy)
+      ).
+
+
+  Definition Proj : { M : mTM (sigX+sigY)^+ 2 & states M -> unit } :=
+    Inject (WriteMove (Some (inr START), R) tt) [|Fin.FS Fin.F1|];;
+    CopySymbols stop_X id;;
+    Inject (
+      (Move _ L tt);;
+      WriteMove (Some (inr START), R) tt
+    ) [|Fin.F1|];;
+    Inject (
+      WriteMove (Some (inr STOP), L) tt;;
+      MoveToSymbol_L stop_Y;;
+      Move _ R tt
+    ) [|Fin.FS Fin.F1|].
+
+  (* Θ (18 + (4+?)*(?+1)*|enocode (fst x)|) *)
+
+
+  Local Lemma CopySymbols_pair_first' (inputX : list sigX) (inputY : list sigY) tltr tl' tr' rs' :
+    tape_local (fst tltr) = map inl (map inl inputX ++ map inr inputY) ++ (inr STOP :: rs') ->
+    (tl', tr') = CopySymbols_Fun stop_X id tltr ->
+    tape_local (tl') = map inl (map inr inputY) ++ (inr STOP :: rs').
+  Proof.
+    intros. destruct inputY as [ | csy inputY'] eqn:E1; cbn in *.
+    - eapply CopySymbols_pair_first; cbn; eauto.
+      + rewrite app_nil_r. intuition. eapply in_map_iff in H1 as (?&<-& (?&<-&?)%in_map_iff). trivial.
+      + trivial.
+    - eapply CopySymbols_pair_first with (str1 := map inl (map inl inputX)); cbn; eauto.
+      + intros x. rewrite !List.map_map. intros (?&<-&?) % in_map_iff. cbn. trivial.
+      + simpl_list. intuition.
+      + now rewrite map_app, <- app_assoc in H.
+  Qed.
+
+  Local Lemma CopySymbols_pair_first'' (inputX : list sigX) (inputY : list sigY) ls m rs tr tl' tr' rs' :
+    m :: rs = map inl (map inl inputX ++ map inr inputY) ++ inr STOP :: rs' ->
+    (tl', tr') = CopySymbols_Fun stop_X id (midtape ls m rs, tr) ->
+    tape_local tl' = map inl (map inr inputY) ++ inr STOP :: rs'.
+  Proof.
+    intros H1 H2. apply (CopySymbols_pair_first' (tltr := (midtape ls m rs, tr)) ltac:(cbn; eapply H1) H2).
+  Qed.
+
+  Local Lemma CopySymbols_pair_second' (inputX : list sigX) (inputY : list sigY) tltr tl' tr' rs' :
+    tape_local (fst tltr) = map inl (map inl inputX ++ map inr inputY) ++ (inr STOP :: rs') ->
+    (tl', tr') = CopySymbols_Fun stop_X id tltr ->
+    left tr' = map inl (map inl (rev inputX)) ++ left (snd tltr).
+  Proof.
+    intros. rewrite !map_rev. destruct inputY as [ | csy inputY'] eqn:E1; cbn in *.
+    - rewrite app_nil_r in H.
+      eapply CopySymbols_pair_second; cbn; eauto.
+      + intros ? (? & <- & (? & <- & ?) % in_map_iff) % in_map_iff. cbn. trivial.
+      + cbn. trivial.
+    - eapply CopySymbols_pair_second with (str1 := map inl (map inl inputX)); cbn; eauto; swap 2 3.
+      + intros x. rewrite !List.map_map. intros (?&<-&?) % in_map_iff. cbn. trivial.
+      + rewrite map_app, <- app_assoc in H. eapply H.
+      + trivial.
+  Qed.
+  
+  Local Lemma CopySymbols_pair_second'' (inputX : list sigX) (inputY : list sigY) ls m rs tr tl' tr' rs' :
+    m :: rs = map inl (map inl inputX ++ map inr inputY) ++ inr STOP :: rs' ->
+    (tl', tr') = CopySymbols_Fun stop_X id (midtape ls m rs, tr) ->
+    left tr' = map inl (map inl (rev inputX)) ++ left tr.
+  Proof.
+    intros H1 H2. apply (CopySymbols_pair_second' (tltr := (midtape ls m rs, tr)) ltac:(cbn; eapply H1) H2).
+  Qed.
+
+  Lemma Proj_WRealise : Proj ⊫ Proj_Rel.
+  Proof.
+    eapply WRealise_monotone.
+    {
+      unfold Proj. do 3 try eapply Seq_WRealise.
+      all: try (eapply Inject_WRealise; [vector_dupfree| ]).
+      3-4: repeat eapply Seq_WRealise.
+      all: try (eapply Realise_WRealise, RealiseIn_Realise;
+                first [ eapply Move_Sem | eapply WriteMove_Sem | eapply Write_Sem ]).
+      - eapply CopySymbols_WRealise.
+      - eapply MoveToSymbol_L_WRealise.
+    }
+    {
+      hnf. intros. hnf. destruct y. intros (inputX, inputY).
+      TMSimp repeat progress simpl_not_in || cbn [Vector.nth] in *.
+      destruct h3; cbn in *; inv H0; [do 2 destruct (encode _); cbn in H3; congruence | ]. clear H1.
+      (*
+      erewrite List.map_app, !List.map_map, <- app_assoc in H3; cbn in H3.
+       *)
+      split.
+      - pose proof CopySymbols_pair_first'' H3 H as L1.
+        destruct h1; cbn in *; try (destruct (encode inputY); cbn in L1; congruence).
+        destruct l; cbn in *.
+        + hnf. do 2 eexists. split; cbn; eauto.
+        + hnf. do 2 eexists. split; cbn; eauto.
+      - pose proof CopySymbols_pair_second'' H3 H as L1. rewrite !map_rev in L1.
+        Set Printing Implicit. cbv [finType_CS] in *. Unset Printing Implicit.
+        rewrite L1 in *.
+        hnf. do 2 eexists. split; cbn.
+        + 
+  Admitted.
+
+End Projection.
+
+
 
 
 (* TODO: Match operator for functions *)
